Iris/Iris/Algebra/View.lean
@@ -312,10 +312,11 @@ instance : UCMRA (View F R) where
 theorem auth_op_auth_eqv : (●V{dq1 • dq2} a : View F R) ≡ (●V{dq1} a) • ●V{dq2} a :=
   ⟨⟨rfl, Agree.idemp.symm⟩, UCMRA.unit_left_id.symm⟩
 
+set_option synthInstance.checkSynthOrder false in
 @[rocq_alias view_auth_dfrac_is_op]
 instance isOp_view_auth_dfrac {dq dq1 dq2 : DFrac F} {a : A}
     [h : IsOp merge dq dq1 dq2] :
-    IsOp io (●V{dq} a : View F R) (●V{dq1} a) (●V{dq2} a) where
+    IsOp io1 (●V{dq} a : View F R) io2 (●V{dq1} a) io3 (●V{dq2} a) where
   is_op := by
     rw [h.is_op]
     apply auth_op_auth_eqv
@@ -359,7 +360,7 @@ instance [CMRA.CoreId b] : CMRA.CoreId ((●V{.discard} a : View F R) • ◯V b
 
 @[rocq_alias view_frag_is_op]
 instance {b b1 b2 : B} [h : IsOp merge b b1 b2] :
-    IsOp io (◯V b : View F R) (◯V b1) (◯V b2) where
+    IsOp io1 (◯V b : View F R) io2 (◯V b1) io3 (◯V b2) where
   is_op := NonExpansive.eqv h.is_op
 
 @[rocq_alias view_auth_dfrac_op_invN]
